src/polytime.lean
@@ -1,5 +1,6 @@
 import data.polynomial.eval
 import time_bound
+import npolynomial
 
 def polytime (c : code) : Prop :=
 ∃ (p : polynomial ℕ), time_bound c (λ n, p.eval n)
@@ -26,10 +27,10 @@ lemma polytime_node {c₁ c₂ : code} : polytime c₁ → polytime c₂ → pol
 | ⟨p₁, e₁⟩ ⟨p₂, e₂⟩ := by { use p₁ + p₂ + 1, convert time_bound_node e₁ e₂, simp, }
 
 lemma polytime_comp {c₁ c₂ : code} : polytime c₁ → polytime c₂ → polytime (code.comp c₁ c₂)
-| ⟨p₁, e₁⟩ ⟨p₂, e₂⟩ := by { use (p₁.comp p₂) + p₂ + 1, convert time_bound_comp e₁ e₂, simp, }
+| ⟨p₁, e₁⟩ ⟨p₂, e₂⟩ := by { use (p₁.comp p₂) + p₂ + 1, convert time_bound_comp (monotone_polynomial_nat _) e₁ e₂, simp, }
 
 lemma polytime_case {c₁ c₂ : code} : polytime c₁ → polytime c₂ → polytime (code.case c₁ c₂)
-| ⟨p₁, e₁⟩ ⟨p₂, e₂⟩ := by { use p₁ + p₂ + 1, convert time_bound_case' e₁ e₂, simp, }
+| ⟨p₁, e₁⟩ ⟨p₂, e₂⟩ := by { use p₁ + p₂ + 1, convert time_bound_case' (monotone_polynomial_nat _) (monotone_polynomial_nat _) e₁ e₂, simp, }
 
 lemma polytime_const (v : ptree) : polytime (code.const v) :=
 by { induction v, { exact polytime_nil, }, apply polytime_node; assumption }
@@ -38,36 +39,36 @@ lemma polytime_ite {c₁ c₂ c₃ : code} (p₁ : polytime c₁) (p₂ : polyti
   polytime (code.ite c₁ c₂ c₃) :=
 polytime_comp (polytime_case p₂ p₃) (polytime_node p₁ polytime_id)
 
-lemma polytime_ite' {c₁ c₂ c₃ : code} (p₁ : polytime c₁) (p₂ p₃ : polynomial ℕ)
-  (hp₂ : ∀ (n : ℕ) (x : ptree), x.sizeof ≤ n → ptree.nil ∈ c₁.eval x → ∃ t ∈ c₂.time x, t ≤ p₂.eval n)
-  (hp₃ : ∀ (n : ℕ) (x : ptree), x.sizeof ≤ n → ptree.nil ∉ c₁.eval x → ∃ t ∈ c₃.time x, t ≤ p₃.eval n) :
-  polytime (c₁.ite c₂ c₃) :=
-begin
-  have ite_dom_univ : (c₁.ite c₂ c₃).eval.dom = set.univ,
-  { rw dom_univ_iff, intro x, rw ite_dom,
-    obtain ⟨r, hr⟩ := part.dom_iff_mem.mp (p₁.dom_univ' x), use [r, hr],
-    split,
-    { rintro rfl, rw [← time_dom_iff_eval_dom, part.dom_iff_mem],
-      obtain ⟨y, hy, _⟩ := hp₂ _ _ rfl.le hr, exact ⟨y, hy⟩, },
-    { intro h, rw [← time_dom_iff_eval_dom, part.dom_iff_mem],
-      obtain ⟨y, hy, _⟩ := hp₃ _ x rfl.le (λ C, h (part.mem_unique hr C)), exact ⟨y, hy⟩, } },
-  have cond_dom_univ : ∀ x, (c₁.eval x).dom := p₁.dom_univ',
-  rcases p₁ with ⟨p₁, e₁⟩,
-  use p₁ + p₂ + p₃ + (polynomial.monomial 1 1) + 3,
-  intros n v hnv,
-  rw [← time_dom_eq_eval_dom, dom_univ_iff] at ite_dom_univ, specialize ite_dom_univ v,
-  rw part.dom_iff_mem at ite_dom_univ, cases ite_dom_univ with t H, use [t, H],
-  specialize cond_dom_univ v, specialize e₁ n v hnv, specialize hp₂ n v hnv, specialize hp₃ n v hnv,
-  obtain ⟨r, hr⟩ := part.dom_iff_mem.mp cond_dom_univ,
-  obtain ⟨tc, htc, tc_le⟩ := e₁,
-  rw ← part.eq_some_iff at hr htc,
-  simp [code.ite, code.time, hr, htc, add_def] at H,
-  rcases H with ⟨t, ht, rfl⟩,
-  suffices : t ≤ p₂.eval n + p₃.eval n,
-  { simp at ⊢, linarith only [this, tc_le, hnv], },
-  split_ifs at ht,
-  { subst h, simp [hr] at hp₂, rcases hp₂ with ⟨t, ht', Ht⟩, cases part.mem_unique ht ht',
-    nlinarith only [Ht], },
-  { rw (@comm _ (=)) at h, simp [hr, h] at hp₃, rcases hp₃ with ⟨t, ht', Ht⟩, cases part.mem_unique ht ht',
-    nlinarith only [Ht], },
-end
+-- lemma polytime_ite' {c₁ c₂ c₃ : code} (p₁ : polytime c₁) (p₂ p₃ : polynomial ℕ)
+--   (hp₂ : ∀ (n : ℕ) (x : ptree), x.sizeof ≤ n → ptree.nil ∈ c₁.eval x → ∃ t ∈ c₂.time x, t ≤ p₂.eval n)
+--   (hp₃ : ∀ (n : ℕ) (x : ptree), x.sizeof ≤ n → ptree.nil ∉ c₁.eval x → ∃ t ∈ c₃.time x, t ≤ p₃.eval n) :
+--   polytime (c₁.ite c₂ c₃) :=
+-- begin
+--   have ite_dom_univ : (c₁.ite c₂ c₃).eval.dom = set.univ,
+--   { rw dom_univ_iff, intro x, rw ite_dom,
+--     obtain ⟨r, hr⟩ := part.dom_iff_mem.mp (p₁.dom_univ' x), use [r, hr],
+--     split,
+--     { rintro rfl, rw [← time_dom_iff_eval_dom, part.dom_iff_mem],
+--       obtain ⟨y, hy, _⟩ := hp₂ _ _ rfl.le hr, exact ⟨y, hy⟩, },
+--     { intro h, rw [← time_dom_iff_eval_dom, part.dom_iff_mem],
+--       obtain ⟨y, hy, _⟩ := hp₃ _ x rfl.le (λ C, h (part.mem_unique hr C)), exact ⟨y, hy⟩, } },
+--   have cond_dom_univ : ∀ x, (c₁.eval x).dom := p₁.dom_univ',
+--   rcases p₁ with ⟨p₁, e₁⟩,
+--   use p₁ + p₂ + p₃ + (polynomial.monomial 1 1) + 3,
+--   intros n v hnv,
+--   rw [← time_dom_eq_eval_dom, dom_univ_iff] at ite_dom_univ, specialize ite_dom_univ v,
+--   rw part.dom_iff_mem at ite_dom_univ, cases ite_dom_univ with t H, use [t, H],
+--   specialize cond_dom_univ v, specialize e₁ n v hnv, specialize hp₂ n v hnv, specialize hp₃ n v hnv,
+--   obtain ⟨r, hr⟩ := part.dom_iff_mem.mp cond_dom_univ,
+--   obtain ⟨tc, htc, tc_le⟩ := e₁,
+--   rw ← part.eq_some_iff at hr htc,
+--   simp [code.ite, code.time, hr, htc, add_def] at H,
+--   rcases H with ⟨t, ht, rfl⟩,
+--   suffices : t ≤ p₂.eval n + p₃.eval n,
+--   { simp at ⊢, linarith only [this, tc_le, hnv], },
+--   split_ifs at ht,
+--   { subst h, simp [hr] at hp₂, rcases hp₂ with ⟨t, ht', Ht⟩, cases part.mem_unique ht ht',
+--     nlinarith only [Ht], },
+--   { rw (@comm _ (=)) at h, simp [hr, h] at hp₃, rcases hp₃ with ⟨t, ht', Ht⟩, cases part.mem_unique ht ht',
+--     nlinarith only [Ht], },
+-- end
